initial version with basic Id example

Main.lean
@@ -1,4 +1,33 @@
-import Hbind
+import HBind.HBind
+import HBind.ElabHdo
 
-def main : IO Unit :=
-  IO.println s!"Hello, {hello}!"
+set_option trace.Elab.do true
+
+-- Elaborating with `hdo` gives us a term based on `hBind`
+def test_IO: IO Unit := hdo
+  IO.println "Lean4"
+  IO.println "hBind"
+  return ()
+#print test_IO
+
+def get_0: Id Nat :=
+  pure 0
+def get_1: Id ((α: Type) → α → α) :=
+  pure @id
+def get_any: Id PUnit.{u+1} :=
+  pure .unit
+
+-- Heterogeneous bind succeeds
+example: Id Unit :=
+  HBind.hBind get_0 fun _ =>
+  HBind.hBind get_1 fun _ =>
+  pure ()
+
+-- If we specify the monad as a polymorphic one, elaboration succeeds
+-- We hacked the universe name so we have to define it
+universe u in
+example: Id Unit := hdo (monad := Id.{u})
+  let _ ← get_0
+  let _ ← get_1
+  let _ ← get_any.{2}
+  get_any.{0}
